theories/Volpic_notation.v
@@ -1,0 +1,19 @@
+Require Import Volpic_preamble.
+
+Declare Scope volpic_notation.
+Open Scope volpic_notation.
+
+Notation "'while' '(' condition ')' 'with' store_name 'upto' loop_limit 'begin' loop_body 'end'" :=
+    (let body := loop_body in 
+        (fix loop (depth : nat) (broken : bool) (VP_store : store) :=
+        match depth with 
+        | O => None
+        | S n' => 
+            if condition VP_store then 
+                loop n' broken (loop_body VP_store)
+            else 
+                (Some VP_store)
+        end) loop_limit false store_name
+    ) : volpic_notation.
+    
+Close Scope volpic_notation.
