theories/palindrome/palindrome.v
@@ -1,0 +1,53 @@
+(*Preamble*)
+Require Import Volpic_preamble.
+Require Import Volpic_notation.
+Require Import String.
+Require Import ZArith.
+Require Import List.
+Require Import Bool.
+Require Import ExtrOcamlBasic.
+Require Import ExtrOcamlString.
+Extraction Language OCaml.
+Open Scope string_scope.
+Open Scope Z_scope.
+Open Scope volpic_notation.
+Import ListNotations.
+
+
+Definition ispalindrome (VP_store: store) := 
+	let VP_poison := false in
+	let (VP_store,VP_poison) := 
+		(if (negb VP_poison) then
+ 			 (update VP_store "VP_result" (VInteger ( 1 )),VP_poison) 
+		else
+ 			(VP_store,true)) in
+	let (VP_store,VP_poison) := 
+		(if (negb VP_poison) then
+ 			 (update VP_store "VP_LEN" (VInteger ( get_int (vp_length VP_store (get_string VP_store "VP_STR")) "VP_result" )),VP_poison) 
+		else
+ 			(VP_store,true)) in
+	let (VP_store,VP_poison) := 
+		(if (negb VP_poison) then
+ 			 (match 
+(let going_up := 1 <? get_int VP_store "VP_LEN" / 2 in
+		let bounds_op := (if going_up then Z.leb else Z.geb) in
+		let iter_op := (if going_up then (Z.add 1) else (Z.sub 1)) in
+		let VP_store := update VP_store "VP_I" (VInteger ( 1 )) in
+while ( fun VP_store => bounds_op (get_int VP_store "VP_I") (get_int VP_store "VP_LEN" / 2) ) with VP_store upto 1000%nat begin fun VP_store => 			let VP_store := if (subscript (get_string VP_store "VP_STR") (get_int VP_store "VP_I") 0 !=? subscript (get_string VP_store "VP_STR") (get_int VP_store "VP_LEN" - get_int VP_store "VP_I" + 1) 0) then
+ 	 ((*Block: next 2 statements*)
+			let VP_store := update VP_store "VP_result" (VInteger ( 0 )) in
+			let VP_broken := true in VP_store) 
+else
+ 	((*nothing and mid-seq*) VP_store) in
+		let VP_store := update VP_store "VP_I" (VInteger (iter_op (get_int VP_store "VP_I"))) in VP_store end) with 
+ 		 | None => (VP_store,true)
+		 | Some VP_store' => (VP_store',VP_poison)
+		 	 end) 
+		else
+ 			(VP_store,true)) in
+VP_store.
+Extraction "palindrome.ml" ispalindrome.
+
+(*Failed to convert $main: Couldn't find key "value" in data list*)
+
+Compute (main fresh_store).
