theories/palindrome/palindrome.p
@@ -1,0 +1,35 @@
+program PalindromeChecker;
+
+// uses
+//   SysUtils;
+
+function IsPalindrome(str: string): boolean;
+var
+  i, len: integer;
+begin
+  IsPalindrome := True;
+
+  len := Length(str);
+  for i := 1 to len div 2 do
+  begin
+    if str[i] <> str[len - i + 1] then
+    begin
+      IsPalindrome := False;
+      break;
+    end;
+  end;
+end;
+
+var
+  inputStr: string;
+begin
+  // Read input from the user
+  Write('Enter a string: ');
+  Readln(inputStr);
+
+  // Check if the input string is a palindrome
+  if IsPalindrome(inputStr) then
+    writeln('The string "', inputStr, '" is a palindrome.')
+  else
+    writeln('The string "', inputStr, '" is not a palindrome.');
+end.
